Phi_System/PhiSem/PhiSem_Min.thy
@@ -17,63 +17,64 @@ subsection \<open>Models\<close>
 subsubsection \<open>Type\<close>
 
 virtual_datatype \<phi>min_ty = \<phi>empty_ty +
-  int     :: nat \<comment> \<open>in unit of bits\<close>
+  T_int     :: nat \<comment> \<open>in unit of bits\<close>
 
 context \<phi>min_ty begin
-abbreviation int where \<open>int \<equiv> int.mk\<close>
+abbreviation int where \<open>int \<equiv> T_int.mk\<close>
 end
+
+debt_axiomatization T_int :: \<open>nat type_entry\<close>
+  where \<phi>min_ty_ax: \<open>\<phi>min_ty TY_CONS_OF T_int\<close>
+
+interpretation \<phi>min_ty TY_CONS_OF _ _ T_int using \<phi>min_ty_ax .
+
+hide_fact \<phi>min_ty_ax \<phi>min_ty_axioms \<phi>min_ty_names_def \<phi>min_ty_def
+  \<phi>min_ty_prjs_axioms \<phi>min_ty_prjs_def \<phi>min_ty.axioms \<phi>min_ty.intro
+  \<phi>min_ty__names.\<phi>min_ty_names_axioms \<phi>min_ty_prjs.axioms
+
 
 subsubsection \<open>Value\<close>
 
-term \<open>Int(a)\<close>
+virtual_datatype \<phi>min_val :: "nonsepable_semigroup" = \<phi>empty_val +
+  V_int     :: \<open>nat \<times> nat\<close> \<comment> \<open>bits \<times> value\<close>
 
-virtual_datatype 'TY \<phi>min_val :: "nonsepable_semigroup" = 'TY \<phi>empty_val +
-  Int     :: \<open>nat \<times> nat\<close> \<comment> \<open>bits \<times> value\<close>
+debt_axiomatization V_int :: \<open>(nat \<times> nat) value_entry\<close>
+  where \<phi>min_val_ax: \<open>\<phi>min_val VAL_CONS_OF V_int\<close>
 
-context \<phi>min_val
-begin
-term int
-end
+interpretation \<phi>min_val VAL_CONS_OF _ _ V_int using \<phi>min_val_ax .
+
+hide_fact \<phi>min_val_ax \<phi>min_val_axioms
+
 
 subsubsection \<open>Resource\<close>
 
 typedef varname = \<open>UNIV::nat set\<close> ..
-type_synonym ('TY,'VAL) R_var = \<open>varname \<rightharpoonup> 'VAL\<close>
+type_synonym R_var = \<open>varname \<rightharpoonup> VAL\<close>
 
 lemma infinite_varname:
   \<open>infinite (UNIV::varname set)\<close>
   by (metis (mono_tags, opaque_lifting) Rep_varname_cases UNIV_I finite_imageI infinite_UNIV_char_0 surj_def)
 
-resource_space ('VAL::nonsepable_semigroup,'TY) \<phi>min_res = ('VAL,'TY) \<phi>empty_res +
-  R_var :: \<open>('TY,'VAL) R_var\<close>
+resource_space \<phi>min_res = \<phi>empty_res +
+  R_var :: R_var
 
-subsubsection \<open>Pure Semantics\<close>
+debt_axiomatization R_var :: \<open>R_var resource_entry\<close>
+  where \<phi>min_res_ax: \<open>\<phi>min_res R_var\<close>
 
-locale \<phi>min_sem =
-  \<phi>min_ty  where CONS_OF   = TY_CONS_OF
-            and TYPE'NAME = \<open>TYPE('TY_N)\<close>
-            and TYPE'REP  = \<open>TYPE('TY)\<close>
-+ V: \<phi>min_val where CONS_OF   = VAL_CONS_OF
-            and TYPE'TY   = \<open>TYPE('TY)\<close>
-            and TYPE'NAME = \<open>TYPE('VAL_N)\<close>
-            and TYPE'REP  = \<open>TYPE('VAL::nonsepable_semigroup)\<close>
-+ R: \<phi>min_res where TYPE'VAL  = \<open>TYPE('VAL)\<close>
-            and TYPE'TY   = \<open>TYPE('TY)\<close>
-            and TYPE'NAME = \<open>TYPE('RES_N)\<close>
-            and TYPE'REP  = \<open>TYPE('RES::sep_algebra)\<close>
-+ \<phi>empty_sem where TYPES = TYPES
-+ \<phi>resource_sem where Resource_Validator = Resource_Validator
-for TYPES :: \<open>(('TY_N \<Rightarrow> 'TY)
-                \<times> ('VAL_N => 'VAL::nonsepable_semigroup)
-                \<times> ('RES_N => 'RES::sep_algebra)) itself\<close>
-+
-assumes WT_int[simp]: \<open>Well_Type (int b)     = { V.Int.mk (b,x)    |x. x < 2 ^ Big b } \<close>
-assumes res_valid_var[simp]: \<open>Resource_Validator R.R_var.name = {R.R_var.inject vars |vars. finite (dom vars)}\<close>
-assumes can_eqcmp_int[simp]: "Can_EqCompare res (V.Int.mk (b1,x1)) (V.Int.mk (b2,x2)) \<longleftrightarrow> b1 = b2"
-assumes eqcmp_int[simp]: "EqCompare (V.Int.mk i1) (V.Int.mk i2) \<longleftrightarrow> i1 = i2"
-assumes zero_int[simp]: \<open>Zero (int b)    = Some (V.Int.mk (b,0))\<close>
+interpretation \<phi>min_res R_var using \<phi>min_res_ax .
 
-begin
+hide_fact \<phi>min_res_ax \<phi>min_res_axioms \<phi>min_res_fields_axioms
+
+
+subsubsection \<open>Semantics\<close>
+
+debt_axiomatization
+    WT_int[simp]: \<open>Well_Type (int b)     = { V_int.mk (b,x)    |x. x < 2 ^ Big b } \<close>
+and res_valid_var[simp]: \<open>Resource_Validator R_var.name =
+                                {R_var.inject vars |vars. finite (dom vars)}\<close>
+and can_eqcmp_int[simp]: "Can_EqCompare res (V_int.mk (b1,x1)) (V_int.mk (b2,x2)) \<longleftrightarrow> b1 = b2"
+and eqcmp_int[simp]: "EqCompare (V_int.mk i1) (V_int.mk i2) \<longleftrightarrow> i1 = i2"
+and  zero_int[simp]: \<open>Zero (int b)    = Some (V_int.mk (b,0))\<close>
 
 lemma Valid_Types[simp]:
   \<open>Valid_Type (int n)\<close>
@@ -81,143 +82,27 @@ lemma Valid_Types[simp]:
   apply simp
   using less_exp by blast
 
-sublocale R_var: partial_map_resource \<open>{vars. finite (dom vars)}\<close> R_var
+interpretation R_var: partial_map_resource \<open>{vars. finite (dom vars)}\<close> R_var
   by (standard; simp add: set_eq_iff image_iff; blast)
 
-end
+subsubsection \<open>Fiction\<close>
 
-fiction_space (in \<phi>min_sem) \<phi>min_fic :: \<open>'RES_N \<Rightarrow> 'RES\<close> =
+fiction_space \<phi>min_fic :: \<open>RES_N \<Rightarrow> RES\<close> =
   FIC_var :: \<open>R_var.raw_basic_fiction \<F>_it\<close>
 
-locale \<phi>min =
-  \<phi>min_sem where TYPES = \<open>TYPE(('TY_N \<Rightarrow> 'TY) \<times> ('VAL_N \<Rightarrow> 'VAL::nonsepable_semigroup)
-                            \<times> ('RES_N \<Rightarrow> 'RES::sep_algebra))\<close>
-+ F: \<phi>min_fic where TYPES = \<open>TYPE(('TY_N \<Rightarrow> 'TY) \<times> ('VAL_N \<Rightarrow> 'VAL::nonsepable_semigroup)
-                            \<times> ('RES_N \<Rightarrow> 'RES::sep_algebra))\<close>
-    and TYPE'FNAME = \<open>TYPE('FIC_N)\<close>
-    and TYPE'FREP = \<open>TYPE('FIC::sep_algebra)\<close> 
-+ \<phi>empty where TYPES = \<open>TYPE(('TY_N \<Rightarrow> 'TY)
-                          \<times> ('VAL_N \<Rightarrow> 'VAL::nonsepable_semigroup)
-                          \<times> ('RES_N \<Rightarrow> 'RES::sep_algebra)
-                          \<times> ('FIC_N \<Rightarrow> 'FIC::sep_algebra))\<close>
-+ fixes TYPES :: \<open>(('TY_N \<Rightarrow> 'TY) \<times> ('VAL_N \<Rightarrow> 'VAL) \<times> ('RES_N \<Rightarrow> 'RES) \<times> ('FIC_N \<Rightarrow> 'FIC)) itself\<close>
-begin
+debt_axiomatization FIC_var :: \<open>R_var fiction_entry\<close>
+  where \<phi>min_fic_ax: \<open>\<phi>min_fic INTERPRET FIC_var\<close>
 
-sublocale FIC_varx: identity_fiction \<open>{vars. finite (dom vars)}\<close> R_var
-    Resource_Validator INTERPRET FIC_var ..
+interpretation \<phi>min_fic INTERPRET FIC_var using \<phi>min_fic_ax .
 
-end
+hide_fact \<phi>min_fic_ax \<phi>min_fic_axioms
 
-print_locale \<phi>min_sem
-ML \<open>Locale.params_of @{theory} @{locale \<phi>min_sem}\<close>
-
-typedecl TY_N
-typedecl TY
-typedecl VAL_N
-typedecl VAL
-typedecl FIC_N
-typedecl FIC
-typedecl RES_N
-typedecl RES
-
-axiomatization where VAL: \<open>OFCLASS(VAL, nonsepable_semigroup_class)\<close>
-and FIC: \<open>OFCLASS(FIC, sep_algebra_class)\<close>
-and RES: \<open>OFCLASS(RES, sep_algebra_class)\<close>
-
-ML \<open>@{term \<open>OFCLASS(FIC, sep_algebra_class)\<close>}\<close>
-ML \<open>Sign.full_bname @{theory} "a"\<close>
-
-setup \<open>Axclass.add_arity @{thm VAL}
-#> Axclass.add_arity @{thm FIC}
-#> Axclass.add_arity @{thm RES}
-\<close>
-
-
-axiomatization \<f>\<i>\<e>\<l>\<d>_int :: "(TY_N, TY, nat) Virtual_Datatype.Field"
-and  T_tup :: "(TY_N, TY, TY list) Virtual_Datatype.Field"
-and  T_array :: "(TY_N, TY, TY \<times> nat) Virtual_Datatype.Field"
-and  \<f>\<i>\<e>\<l>\<d>_Int :: "(VAL_N, VAL, nat \<times> nat) Virtual_Datatype.Field"
-and  V_Tup :: "(VAL_N, VAL, VAL list) Virtual_Datatype.Field"
-and  V_Array :: "(VAL_N, VAL, TY \<times> VAL list) Virtual_Datatype.Field"
-and  INTERPRET :: "FIC_N \<Rightarrow> (FIC, RES_N \<Rightarrow> RES) interp"
-and  FIC_var :: "(FIC_N, FIC, varname \<Rightarrow> VAL option) Virtual_Datatype.Field"
-and  TY_CONS_OF :: "TY \<Rightarrow> TY_N"
-and  VAL_CONS_OF :: "VAL \<Rightarrow> VAL_N"
-and  Resource_Validator :: "RES_N \<Rightarrow> RES set"
-and  Well_Type :: "TY \<Rightarrow> VAL set"
-and  Can_EqCompare :: "(RES_N \<Rightarrow> RES) \<Rightarrow> VAL \<Rightarrow> VAL \<Rightarrow> bool"
-and  EqCompare :: "VAL \<Rightarrow> VAL \<Rightarrow> bool"
-and  Zero :: "TY \<Rightarrow> VAL option"
-and  R_var :: "(RES_N, RES, varname \<Rightarrow> VAL option) Virtual_Datatype.Field"
-where XXX: \<open>\<phi>min_sem \<f>\<i>\<e>\<l>\<d>_int \<f>\<i>\<e>\<l>\<d>_Int R_var TY_CONS_OF VAL_CONS_OF Resource_Validator Well_Type Can_EqCompare
-      EqCompare Zero\<close>
-
-print_locale \<phi>min_sem
-
-global_interpretation mm: \<phi>min_sem \<f>\<i>\<e>\<l>\<d>_int \<f>\<i>\<e>\<l>\<d>_Int R_var TY_CONS_OF VAL_CONS_OF Resource_Validator Well_Type Can_EqCompare
-      EqCompare Zero
-  using XXX .
-
-
-
-
-axiomatization \<f>\<i>\<e>\<l>\<d>_int :: "(TY_N, TY, nat) Virtual_Datatype.Field"
-and  T_tup :: "(TY_N, TY, TY list) Virtual_Datatype.Field"
-and  T_array :: "(TY_N, TY, TY \<times> nat) Virtual_Datatype.Field"
-and  \<f>\<i>\<e>\<l>\<d>_Int :: "(VAL_N, VAL, nat \<times> nat) Virtual_Datatype.Field"
-and  V_Tup :: "(VAL_N, VAL, VAL list) Virtual_Datatype.Field"
-and  V_Array :: "(VAL_N, VAL, TY \<times> VAL list) Virtual_Datatype.Field"
-and  INTERPRET :: "FIC_N \<Rightarrow> (FIC, RES_N \<Rightarrow> RES) interp"
-and  FIC_var :: "(FIC_N, FIC, varname \<Rightarrow> VAL option) Virtual_Datatype.Field"
-and  TY_CONS_OF :: "TY \<Rightarrow> TY_N"
-and  VAL_CONS_OF :: "VAL \<Rightarrow> VAL_N"
-and  Resource_Validator :: "RES_N \<Rightarrow> RES set"
-and  Well_Type :: "TY \<Rightarrow> VAL set"
-and  Can_EqCompare :: "(RES_N \<Rightarrow> RES) \<Rightarrow> VAL \<Rightarrow> VAL \<Rightarrow> bool"
-and  EqCompare :: "VAL \<Rightarrow> VAL \<Rightarrow> bool"
-and  Zero :: "TY \<Rightarrow> VAL option"
-and  R_var :: "(RES_N, RES, varname \<Rightarrow> VAL option) Virtual_Datatype.Field"
-where XXX: \<open>\<phi>min \<f>\<i>\<e>\<l>\<d>_int \<f>\<i>\<e>\<l>\<d>_Int R_var TY_CONS_OF VAL_CONS_OF Resource_Validator Well_Type Can_EqCompare
-      EqCompare Zero INTERPRET FIC_var\<close>
-
-print_locale \<phi>min
-
-global_interpretation mm: \<phi>min \<f>\<i>\<e>\<l>\<d>_int \<f>\<i>\<e>\<l>\<d>_Int R_var TY_CONS_OF VAL_CONS_OF Resource_Validator Well_Type Can_EqCompare
-      EqCompare Zero INTERPRET FIC_var
-  using XXX .
-
-
-
-
-axiomatization T_int :: "(TY_N, TY, nat) Virtual_Datatype.Field"
-and  T_tup :: "(TY_N, TY, TY list) Virtual_Datatype.Field"
-and  T_array :: "(TY_N, TY, TY \<times> nat) Virtual_Datatype.Field"
-and  V_int :: "(VAL_N, VAL, nat \<times> nat) Virtual_Datatype.Field"
-and  V_Tup :: "(VAL_N, VAL, VAL list) Virtual_Datatype.Field"
-and  V_Array :: "(VAL_N, VAL, TY \<times> VAL list) Virtual_Datatype.Field"
-and  INTERPRET :: "FIC_N \<Rightarrow> (FIC, RES_N \<Rightarrow> RES) interp"
-and  FIC_var :: "(FIC_N, FIC, varname \<Rightarrow> VAL option) Virtual_Datatype.Field"
-and  TY_CONS_OF :: "TY \<Rightarrow> TY_N"
-and  VAL_CONS_OF :: "VAL \<Rightarrow> VAL_N"
-and  Resource_Validator :: "RES_N \<Rightarrow> RES set"
-and  Well_Type :: "TY \<Rightarrow> VAL set"
-and  Can_EqCompare :: "(RES_N \<Rightarrow> RES) \<Rightarrow> VAL \<Rightarrow> VAL \<Rightarrow> bool"
-and  EqCompare :: "VAL \<Rightarrow> VAL \<Rightarrow> bool"
-and  Zero :: "TY \<Rightarrow> VAL option"
-and  R_var :: "(RES_N, RES, varname \<Rightarrow> VAL option) Virtual_Datatype.Field"
-where XXX: \<open>\<phi>min TY_CONS_OF VAL_CONS_OF Resource_Validator Well_Type Can_EqCompare
-      EqCompare Zero \<f>\<i>\<e>\<l>\<d>_int \<f>\<i>\<e>\<l>\<d>_Int R_var INTERPRET FIC_var\<close>
-
-interpretation mm: \<phi>min TY_CONS_OF VAL_CONS_OF Resource_Validator Well_Type Can_EqCompare
-      EqCompare Zero T_int V_int R_var INTERPRET FIC_var
-  using XXX .
+interpretation FIC_var: identity_fiction \<open>{vars. finite (dom vars)}\<close> R_var FIC_var ..
 
 
 section \<open>\<phi>-Types\<close>
 
 \<phi>overloads nat and int
-
-context \<phi>min_sem begin
 
 subsection \<open>Integer\<close>
 
@@ -225,21 +110,20 @@ subsubsection \<open>Natural Nmbers\<close>
 
 paragraph \<open>Natural Number\<close>
 
-definition \<phi>Nat :: "nat \<Rightarrow> ('VAL, nat) \<phi>" ("\<nat>[_]")
-  where "\<nat>[b] x = (if x < 2^b then { V.Int.mk (b,x) } else {})"
+definition \<phi>Nat :: "nat \<Rightarrow> (VAL, nat) \<phi>" ("\<nat>[_]")
+  where "\<nat>[b] x = (if x < 2^b then { V_int.mk (b,x) } else {})"
 
 (* abbreviation \<open>Size \<equiv> \<nat>[addrspace_bits]\<close> *)
 
 lemma \<phi>Nat_expn[\<phi>expns]:
-  "p \<in> (x \<Ztypecolon> \<nat>[b]) \<longleftrightarrow> (p = V.Int.mk (b,x)) \<and> x < 2 ^ Big b"
+  "p \<in> (x \<Ztypecolon> \<nat>[b]) \<longleftrightarrow> (p = V_int.mk (b,x)) \<and> x < 2 ^ Big b"
   unfolding \<phi>Type_def Big_def by (simp add: \<phi>Nat_def)
 
 lemma \<phi>Nat_elim[elim!,\<phi>inhabitance_rule]:
   "Inhabited (x \<Ztypecolon> \<nat>[b]) \<Longrightarrow> (x < 2 ^ Big b \<Longrightarrow> C) \<Longrightarrow> C"
   unfolding Inhabited_def by (simp add: \<phi>expns)
 
-lemma
-  \<open>Inhabited (x \<Ztypecolon> \<nat>[b]) \<longleftrightarrow> x < 2^Big b\<close>
+lemma \<open>Inhabited (x \<Ztypecolon> \<nat>[b]) \<longleftrightarrow> x < 2^Big b\<close>
   unfolding Inhabited_def by (simp add: \<phi>expns)
 
 lemma \<phi>Nat_semty[\<phi>reason for \<open>\<phi>SemType (?x \<Ztypecolon> \<nat>[?b]) ?ty\<close>]:
@@ -260,42 +144,40 @@ lemma [\<phi>reason]:
 
 paragraph \<open>Rounded Natural Number\<close>
 
-definition \<phi>NatRound :: "nat \<Rightarrow> ('VAL, nat) \<phi>" ("\<nat>\<^sup>r[_]")
-  where "\<nat>\<^sup>r[b] x = { V.Int.mk (b, (x mod 2 ^ Big b)) }"
+definition \<phi>NatRound :: "nat \<Rightarrow> (VAL, nat) \<phi>" ("\<nat>\<^sup>r[_]")
+  where "\<nat>\<^sup>r[b] x = { V_int.mk (b, (x mod 2 ^ Big b)) }"
 
 lemma \<phi>NatRound_expn[\<phi>expns]:
-  "p \<in> (x \<Ztypecolon> \<nat>\<^sup>r[b]) \<longleftrightarrow> p = V.Int.mk (b, (x mod 2 ^ Big b))"
+  "p \<in> (x \<Ztypecolon> \<nat>\<^sup>r[b]) \<longleftrightarrow> p = V_int.mk (b, (x mod 2 ^ Big b))"
   unfolding \<phi>Type_def \<phi>NatRound_def by simp
 
-lemma
-  \<open>Inhabited (x \<Ztypecolon> \<nat>\<^sup>r[b]) \<longleftrightarrow> True\<close>
+lemma \<open>Inhabited (x \<Ztypecolon> \<nat>\<^sup>r[b]) \<longleftrightarrow> True\<close>
   unfolding Inhabited_def by (auto simp add: \<phi>expns)
 
-lemma [\<phi>reason for \<open>\<phi>Zero (int.mk ?b) \<nat>\<^sup>r[?b] ?z\<close>]:
-  "\<phi>Zero (int.mk b) (\<nat>\<^sup>r[b]) 0"
+lemma [\<phi>reason for \<open>\<phi>Zero (int ?b) \<nat>\<^sup>r[?b] ?z\<close>]:
+  "\<phi>Zero (int b) (\<nat>\<^sup>r[b]) 0"
   unfolding \<phi>Zero_def by (simp add: \<phi>expns)
 
 lemma \<phi>NatRound_semty[\<phi>reason for \<open>\<phi>SemType (?x \<Ztypecolon> \<nat>\<^sup>r[?b]) ?ty\<close>]:
   \<open>\<phi>SemType (x \<Ztypecolon> \<nat>\<^sup>r[b]) (int b)\<close>
   unfolding \<phi>SemType_def subset_iff by (simp add: \<phi>expns)
 
+
 subsubsection \<open>Integer in the normal sense\<close>
 
-
-definition \<phi>Int :: "nat \<Rightarrow> ('VAL, int) \<phi>" ("\<int>[_]")
+definition \<phi>Int :: "nat \<Rightarrow> (VAL, int) \<phi>" ("\<int>[_]")
   where "\<phi>Int b x =(if x < 2^(b - 1) \<and> -(2^(b-1)) \<le> x \<and> (b = 0 \<longrightarrow> x = 0)
-                    then { V.Int.mk (b, (if x \<ge> 0 then nat x else nat (2^b + x))) }
+                    then { V_int.mk (b, (if x \<ge> 0 then nat x else nat (2^b + x))) }
                     else {})"
 
 lemma \<phi>Int_expn[\<phi>expns]:
-  "p \<in> (x \<Ztypecolon> \<int>[b]) \<longleftrightarrow> p = V.Int.mk (b, (if x \<ge> 0 then nat x else nat (2^b + x)))
+  "p \<in> (x \<Ztypecolon> \<int>[b]) \<longleftrightarrow> p = V_int.mk (b, (if x \<ge> 0 then nat x else nat (2^b + x)))
                       \<and> x < 2^(b - 1) \<and> -(2^(b-1)) \<le> x \<and> (b = 0 \<longrightarrow> x = 0)"
   unfolding \<phi>Type_def by (simp add: \<phi>Int_def)
 
 lemma \<phi>Int_inhabited[elim!,\<phi>inhabitance_rule]:
   "Inhabited (x \<Ztypecolon> \<int>[b]) \<Longrightarrow> (x < 2^(b - 1) \<and> -(2^(b-1)) \<le> x \<and> (b = 0 \<longrightarrow> x = 0) \<Longrightarrow> C) \<Longrightarrow> C"
   unfolding Inhabited_def by (simp add: \<phi>expns) 
-
 
 lemma [simp]: \<open>- (2^(b - 1)) \<le> x \<Longrightarrow> 0 \<le> 2 ^ b + x\<close> for x :: int
   by (smt (verit, best) diff_le_self power_increasing_iff)
@@ -304,8 +186,8 @@ lemma [\<phi>reason for \<open>\<phi>Equal \<int>[b] ?c ?eq\<close>]:
     "\<phi>Equal \<int>[b] (\<lambda>x y. True) (=)"
   unfolding \<phi>Equal_def by (cases b) (auto simp add: \<phi>expns eq_nat_nat_iff)
 
-lemma [\<phi>reason for \<open>\<phi>Zero (int.mk ?b) \<int>[?b] ?x\<close>]:
-    "\<phi>Zero (int.mk b) \<int>[b] 0"
+lemma [\<phi>reason for \<open>\<phi>Zero (int ?b) \<int>[?b] ?x\<close>]:
+    "\<phi>Zero (int b) \<int>[b] 0"
   unfolding \<phi>Zero_def by (simp add: \<phi>expns)
 
 lemma \<phi>Int_semty[\<phi>reason for \<open>\<phi>SemType (?x \<Ztypecolon> \<int>[?b]) ?ty\<close>]:
@@ -336,11 +218,11 @@ subsubsection \<open>Boolean\<close>
   then show ?thesis  by auto
 qed *)
 
-definition \<phi>Bool :: "('VAL, bool) \<phi>" ("\<bool>")
-  where "\<bool> x = { V.Int.mk (1, (if x then 1 else 0)) }"
+definition \<phi>Bool :: "(VAL, bool) \<phi>" ("\<bool>")
+  where "\<bool> x = { V_int.mk (1, (if x then 1 else 0)) }"
 
 lemma \<phi>Bool_expn[\<phi>expns]:
-  " p \<in> (x \<Ztypecolon> \<bool>) \<longleftrightarrow> p = V.Int.mk (1, (if x then 1 else 0))"
+  " p \<in> (x \<Ztypecolon> \<bool>) \<longleftrightarrow> p = V_int.mk (1, (if x then 1 else 0))"
   unfolding \<phi>Type_def \<phi>Bool_def by simp
 
 lemma \<phi>Bool_inhabited[\<phi>inhabitance_rule, elim!]:
@@ -363,17 +245,12 @@ lemma [\<phi>reason]:
   \<open>is_singleton (x \<Ztypecolon> \<bool>)\<close>
   by (rule is_singletonI''; simp add: \<phi>expns)
 
-
 abbreviation \<open>Predicate_About x \<equiv> (\<bool> <func-over> x)\<close>
-
-end
 
 
 subsection \<open>Variable\<close>
 
-context \<phi>min begin
-
-abbreviation Var :: \<open>varname \<Rightarrow> ('VAL,'a) \<phi> \<Rightarrow> 'a \<Rightarrow> ('FIC_N \<Rightarrow> 'FIC) set\<close>
+abbreviation Var :: \<open>varname \<Rightarrow> (VAL,'a) \<phi> \<Rightarrow> 'a \<Rightarrow> assn\<close>
   where \<open>Var vname T \<equiv> (FIC_var.\<phi> (vname \<^bold>\<rightarrow> \<black_circle> T))\<close>
 
 lemma Var_inhabited[\<phi>inhabitance_rule,elim!]:
@@ -420,7 +297,6 @@ lemma [\<phi>reason 1300 for \<open>\<^bold>v\<^bold>i\<^bold>e\<^bold>w ?R \<he
   unfolding GOAL_CTXT_def FOCUS_TAG_def
   by (simp add: Var_view_shift \<phi>frame_view view_shift_id) 
 
-
 lemma Var_simp_cong:
   \<open> (x \<Ztypecolon> T) = (x' \<Ztypecolon> T')
 \<Longrightarrow> (x \<Ztypecolon> Var v T) = (x' \<Ztypecolon> Var v T')\<close>
@@ -429,6 +305,7 @@ lemma Var_simp_cong:
 simproc_setup Var_simp_cong ("x \<Ztypecolon> Var v T") = \<open>
   K (NuSimpCong.simproc @{thm Var_simp_cong[folded atomize_eq]})
 \<close>
+
 
 subsubsection \<open>Rules\<close>
 
@@ -487,32 +364,28 @@ lemma [\<phi>reason 2000 for \<open>
   using "\<phi>cast_P" Var_cast_\<phi>app[unfolded Argument_def] implies_left_prod
   by (metis Var_subty)
 
-end
-
 
 section \<open>Instructions\<close>
-
-context \<phi>min_sem begin
 
 subsection \<open>Arithmetic Operations\<close>
 
 subsubsection \<open>Integer arithmetic\<close>
 
-definition op_const_int :: "nat \<Rightarrow> nat \<Rightarrow> ('VAL,'VAL,'RES_N,'RES) proc"
-  where "op_const_int bits const = Return (sem_value (V.Int.mk (bits,const)))"
+definition op_const_int :: "nat \<Rightarrow> nat \<Rightarrow> VAL proc"
+  where "op_const_int bits const = Return (sem_value (V_int.mk (bits,const)))"
 
-(* definition op_const_size_t :: "nat \<Rightarrow> ('VAL,'VAL,'RES_N,'RES) proc"
+(* definition op_const_size_t :: "nat \<Rightarrow> (VAL,VAL,'RES_N,'RES) proc"
   where "op_const_size_t c = \<phi>M_assume (c < 2 ^ addrspace_bits)
-                          \<ggreater> Return (sem_value (V.Int.mk (addrspace_bits,c)))"
+                          \<ggreater> Return (sem_value (V_int.mk (addrspace_bits,c)))"
   \<comment> \<open> `op_const_size_t` checks the overflow during the compilation towards certain decided platform.  \<close>
 *)
 
-definition op_add :: "nat \<Rightarrow> ('VAL \<times> 'VAL, 'VAL, 'VAL, 'RES_N, 'RES) proc'"
+definition op_add :: "nat \<Rightarrow> (VAL \<times> VAL, VAL) proc'"
   where "op_add bits =
       \<phi>M_caseV (\<lambda>vb va.
-      \<phi>M_getV (int bits) (snd o V.Int.dest) vb (\<lambda>val_b.
-      \<phi>M_getV (int bits) (snd o V.Int.dest) va (\<lambda>val_a.
-      Return (sem_value (V.Int.mk (bits, ((val_a + val_b) mod 2^bits))))
+      \<phi>M_getV (int bits) (snd o V_int.dest) vb (\<lambda>val_b.
+      \<phi>M_getV (int bits) (snd o V_int.dest) va (\<lambda>val_a.
+      Return (sem_value (V_int.mk (bits, ((val_a + val_b) mod 2^bits))))
   )))"
 
 
@@ -530,92 +403,92 @@ definition op_add :: "nat \<Rightarrow> ('VAL \<times> 'VAL, 'VAL, 'VAL, 'RES_N,
 \<Longrightarrow> \<^bold>p\<^bold>r\<^bold>o\<^bold>c (left \<ggreater> right \<ggreater> op_add b) \<lbrace> R1 \<longmapsto> R3\<heavy_comma> SYNTHESIS x + y \<Ztypecolon> \<nat>[b] \<rbrace>\<close>
   apply (\<phi>reason, assumption) *)
 
-definition op_sub :: "nat \<Rightarrow> ('VAL \<times> 'VAL, 'VAL, 'VAL, 'RES_N, 'RES) proc'"
+definition op_sub :: "nat \<Rightarrow> (VAL \<times> VAL, VAL) proc'"
   where "op_sub bits =
       \<phi>M_caseV (\<lambda>va vb.
-      \<phi>M_getV (int bits) (snd o V.Int.dest) va (\<lambda>val_a.
-      \<phi>M_getV (int bits) (snd o V.Int.dest) vb (\<lambda>val_b.
-      Return (sem_value (V.Int.mk (bits, ((2^bits + val_b - val_a) mod 2^bits))))
+      \<phi>M_getV (int bits) (snd o V_int.dest) va (\<lambda>val_a.
+      \<phi>M_getV (int bits) (snd o V_int.dest) vb (\<lambda>val_b.
+      Return (sem_value (V_int.mk (bits, ((2^bits + val_b - val_a) mod 2^bits))))
   )))"
 
-definition op_umul :: "nat \<Rightarrow> ('VAL \<times> 'VAL, 'VAL, 'VAL, 'RES_N, 'RES) proc'"
+definition op_umul :: "nat \<Rightarrow> (VAL \<times> VAL, VAL) proc'"
   where "op_umul bits =
       \<phi>M_caseV (\<lambda>va vb.
-      \<phi>M_getV (int bits) (snd o V.Int.dest) va (\<lambda>val_a.
-      \<phi>M_getV (int bits) (snd o V.Int.dest) vb (\<lambda>val_b.
-      Return (sem_value (V.Int.mk (bits, ((val_b * val_a) mod 2^bits))))
+      \<phi>M_getV (int bits) (snd o V_int.dest) va (\<lambda>val_a.
+      \<phi>M_getV (int bits) (snd o V_int.dest) vb (\<lambda>val_b.
+      Return (sem_value (V_int.mk (bits, ((val_b * val_a) mod 2^bits))))
   )))"
 
-definition op_udiv :: "nat \<Rightarrow> ('VAL \<times> 'VAL, 'VAL, 'VAL, 'RES_N, 'RES) proc'"
+definition op_udiv :: "nat \<Rightarrow> (VAL \<times> VAL, VAL) proc'"
   where "op_udiv bits =
       \<phi>M_caseV (\<lambda>va vb.
-      \<phi>M_getV (int bits) (snd o V.Int.dest) va (\<lambda>val_a.
-      \<phi>M_getV (int bits) (snd o V.Int.dest) vb (\<lambda>val_b.
-      Return (sem_value (V.Int.mk (bits, (val_b div val_a))))
+      \<phi>M_getV (int bits) (snd o V_int.dest) va (\<lambda>val_a.
+      \<phi>M_getV (int bits) (snd o V_int.dest) vb (\<lambda>val_b.
+      Return (sem_value (V_int.mk (bits, (val_b div val_a))))
   )))"
 
-definition op_lshr :: "nat \<Rightarrow> nat \<Rightarrow> ('VAL \<times> 'VAL, 'VAL, 'VAL, 'RES_N, 'RES) proc'"
+definition op_lshr :: "nat \<Rightarrow> nat \<Rightarrow> (VAL \<times> VAL, VAL) proc'"
   where "op_lshr b_b b_a =
       \<phi>M_caseV (\<lambda>va vb.
-      \<phi>M_getV (int b_a) (snd o V.Int.dest) va (\<lambda>val_a.
-      \<phi>M_getV (int b_b) (snd o V.Int.dest) vb (\<lambda>val_b.
-      Return (sem_value (V.Int.mk (b_b, (val_b div 2 ^ val_a))))
+      \<phi>M_getV (int b_a) (snd o V_int.dest) va (\<lambda>val_a.
+      \<phi>M_getV (int b_b) (snd o V_int.dest) vb (\<lambda>val_b.
+      Return (sem_value (V_int.mk (b_b, (val_b div 2 ^ val_a))))
   )))"
 
-definition op_lshl :: "nat \<Rightarrow> nat \<Rightarrow> ('VAL \<times> 'VAL, 'VAL, 'VAL, 'RES_N, 'RES) proc'"
+definition op_lshl :: "nat \<Rightarrow> nat \<Rightarrow> (VAL \<times> VAL, VAL) proc'"
   where "op_lshl b_b b_a =
       \<phi>M_caseV (\<lambda>va vb.
-      \<phi>M_getV (int b_a) (snd o V.Int.dest) va (\<lambda>val_a.
-      \<phi>M_getV (int b_b) (snd o V.Int.dest) vb (\<lambda>val_b.
-      Return (sem_value (V.Int.mk (b_b, (val_b * 2 ^ val_a))))
+      \<phi>M_getV (int b_a) (snd o V_int.dest) va (\<lambda>val_a.
+      \<phi>M_getV (int b_b) (snd o V_int.dest) vb (\<lambda>val_b.
+      Return (sem_value (V_int.mk (b_b, (val_b * 2 ^ val_a))))
   )))"
 
-definition op_lt :: "nat \<Rightarrow> ('VAL \<times> 'VAL, 'VAL,'VAL,'RES_N,'RES) proc'"
+definition op_lt :: "nat \<Rightarrow> (VAL \<times> VAL, VAL) proc'"
   where "op_lt bits =
       \<phi>M_caseV (\<lambda>va vb.
-      \<phi>M_getV (int bits) (snd o V.Int.dest) va (\<lambda>val_a.
-      \<phi>M_getV (int bits) (snd o V.Int.dest) vb (\<lambda>val_b.
-      Return (sem_value (V.Int.mk (1, (if val_b < val_a then 1 else 0))))
+      \<phi>M_getV (int bits) (snd o V_int.dest) va (\<lambda>val_a.
+      \<phi>M_getV (int bits) (snd o V_int.dest) vb (\<lambda>val_b.
+      Return (sem_value (V_int.mk (1, (if val_b < val_a then 1 else 0))))
   )))"
 
-definition op_le :: "nat \<Rightarrow> ('VAL \<times> 'VAL, 'VAL,'VAL,'RES_N,'RES) proc'"
+definition op_le :: "nat \<Rightarrow> (VAL \<times> VAL, VAL) proc'"
   where "op_le bits =
       \<phi>M_caseV (\<lambda>va vb.
-      \<phi>M_getV (int bits) (snd o V.Int.dest) va (\<lambda>val_a.
-      \<phi>M_getV (int bits) (snd o V.Int.dest) vb (\<lambda>val_b.
-      Return (sem_value (V.Int.mk (1, (if val_b \<le> val_a then 1 else 0))))
+      \<phi>M_getV (int bits) (snd o V_int.dest) va (\<lambda>val_a.
+      \<phi>M_getV (int bits) (snd o V_int.dest) vb (\<lambda>val_b.
+      Return (sem_value (V_int.mk (1, (if val_b \<le> val_a then 1 else 0))))
   )))"
 
 
-definition op_not :: "('VAL, 'VAL,'VAL,'RES_N,'RES) proc'"
+definition op_not :: "(VAL, VAL) proc'"
   where "op_not v =
-    \<phi>M_getV (int 1) (snd o V.Int.dest) v (\<lambda>v.
-    Return (sem_value (V.Int.mk (1, 1 - v)))
+    \<phi>M_getV (int 1) (snd o V_int.dest) v (\<lambda>v.
+    Return (sem_value (V_int.mk (1, 1 - v)))
   )"
 
-definition op_and :: "('VAL \<times> 'VAL, 'VAL,'VAL,'RES_N,'RES) proc'"
+definition op_and :: "(VAL \<times> VAL, VAL) proc'"
   where "op_and =
     \<phi>M_caseV (\<lambda>va vb.
-    \<phi>M_getV (int 1) (snd o V.Int.dest) va (\<lambda>v.
-    \<phi>M_getV (int 1) (snd o V.Int.dest) vb (\<lambda>u.
-    Return (sem_value (V.Int.mk (1, v+u-1)))
+    \<phi>M_getV (int 1) (snd o V_int.dest) va (\<lambda>v.
+    \<phi>M_getV (int 1) (snd o V_int.dest) vb (\<lambda>u.
+    Return (sem_value (V_int.mk (1, v+u-1)))
   )))"
 
-definition op_or :: "('VAL \<times> 'VAL, 'VAL,'VAL,'RES_N,'RES) proc'"
+definition op_or :: "(VAL \<times> VAL, VAL) proc'"
   where "op_or =
     \<phi>M_caseV (\<lambda>va vb.
-    \<phi>M_getV (int 1) (snd o V.Int.dest) va (\<lambda>v.
-    \<phi>M_getV (int 1) (snd o V.Int.dest) vb (\<lambda>u.
-    Return (sem_value (V.Int.mk (1, min 1 (v+u))))
+    \<phi>M_getV (int 1) (snd o V_int.dest) va (\<lambda>v.
+    \<phi>M_getV (int 1) (snd o V_int.dest) vb (\<lambda>u.
+    Return (sem_value (V_int.mk (1, min 1 (v+u))))
   )))"
 
-definition op_equal :: "'TY \<Rightarrow> ('VAL \<times> 'VAL, 'VAL,'VAL,'RES_N,'RES) proc'"
+definition op_equal :: "TY \<Rightarrow> (VAL \<times> VAL, VAL) proc'"
   where "op_equal TY =
     \<phi>M_caseV (\<lambda>va vb.
     \<phi>M_getV TY id va (\<lambda>v.
     \<phi>M_getV TY id vb (\<lambda>u.
     (\<lambda>res. \<phi>M_assert (Can_EqCompare res u v) res) \<ggreater>
-    Return (sem_value (V.Int.mk (1, (if EqCompare u v then 1 else 0))))
+    Return (sem_value (V_int.mk (1, (if EqCompare u v then 1 else 0))))
 )))"
 
 
@@ -623,32 +496,29 @@ definition op_equal :: "'TY \<Rightarrow> ('VAL \<times> 'VAL, 'VAL,'VAL,'RES_N,
 
 subsection \<open>Variable Operations\<close>
 
-definition \<phi>M_get_var
-    :: "varname \<Rightarrow> 'TY \<Rightarrow> ('VAL \<Rightarrow> ('ret,'VAL,'RES_N,'RES) proc) \<Rightarrow> ('ret,'VAL,'RES_N,'RES) proc"
+definition \<phi>M_get_var :: "varname \<Rightarrow> TY \<Rightarrow> (VAL \<Rightarrow> 'ret proc) \<Rightarrow> 'ret proc"
   where "\<phi>M_get_var vname TY F = R_var.\<phi>R_get_res_entry vname (\<lambda>val.
             \<phi>M_assert (val \<in> Well_Type TY) \<ggreater> F val)"
 
-definition op_get_var :: "varname \<Rightarrow> 'TY \<Rightarrow> ('VAL,'VAL,'RES_N,'RES) proc"
+definition op_get_var :: "varname \<Rightarrow> TY \<Rightarrow> VAL proc"
   where "op_get_var vname TY = \<phi>M_get_var vname TY (\<lambda>x. Return (sem_value x))"
 
-definition op_set_var :: "varname \<Rightarrow> 'TY \<Rightarrow> ('VAL, unit,'VAL,'RES_N,'RES) proc'"
+definition op_set_var :: "varname \<Rightarrow> TY \<Rightarrow> (VAL,unit) proc'"
   where "op_set_var vname TY v =
           \<phi>M_getV TY id v (\<lambda>v.
           \<phi>M_get_var vname TY (\<lambda>_.
           R_var.\<phi>R_set_res (\<lambda>f. f(vname := Some v))))"
 
-definition op_free_var :: "varname \<Rightarrow> (unit,'VAL,'RES_N,'RES) proc"
+definition op_free_var :: "varname \<Rightarrow> unit proc"
   where "op_free_var vname = R_var.\<phi>R_set_res (\<lambda>f. f(vname := None))"
 
-definition op_var_scope' :: "'TY
-                          \<Rightarrow> (varname \<Rightarrow> ('ret,'VAL,'RES_N,'RES) proc)
-                          \<Rightarrow> ('VAL,'ret,'VAL,'RES_N,'RES) proc'"
+definition op_var_scope' :: "TY \<Rightarrow> (varname \<Rightarrow> 'ret proc) \<Rightarrow> (VAL,'ret) proc'"
   where "op_var_scope' TY F v =
     \<phi>M_getV TY id v (\<lambda>v.
     R_var.\<phi>R_allocate_res_entry (\<lambda>_. True) (Some v) F
   )"
 
-lemma (in \<phi>min) \<phi>M_get_var[intro!]:
+lemma \<phi>M_get_var[intro!]:
   \<open> v \<in> Well_Type TY
 \<Longrightarrow> \<^bold>p\<^bold>r\<^bold>o\<^bold>c F v \<lbrace> v \<Ztypecolon> Var vname Identity \<longmapsto> Y \<rbrace>
 \<Longrightarrow> \<^bold>p\<^bold>r\<^bold>o\<^bold>c \<phi>M_get_var vname TY F \<lbrace> v \<Ztypecolon> Var vname Identity \<longmapsto> Y \<rbrace>\<close>
@@ -656,7 +526,7 @@ lemma (in \<phi>min) \<phi>M_get_var[intro!]:
   by (clarsimp simp add: \<phi>expns FIC_var.expand simp del: set_mult_expn del: subsetI;
       rule R_var.\<phi>R_get_res_entry[where v=v]; simp)
 
-lemma (in \<phi>min) \<phi>M_set_var[intro!]:
+lemma \<phi>M_set_var[intro!]:
   \<open>\<^bold>p\<^bold>r\<^bold>o\<^bold>c R_var.\<phi>R_set_res (\<lambda>f. f(vname \<mapsto> u)) \<lbrace> v \<Ztypecolon> Var vname Identity \<longmapsto> \<lambda>_. u \<Ztypecolon> Var vname Identity \<rbrace>\<close>
   unfolding \<phi>Procedure_\<phi>Res_Spec
   thm  FIC_var.expand_subj[where x=\<open>1(vname \<mapsto> u)\<close>]
@@ -665,23 +535,21 @@ lemma (in \<phi>min) \<phi>M_set_var[intro!]:
                simp del: set_mult_expn del: subsetI;
       rule R_var.\<phi>R_set_res[where P=\<open>\<lambda>_. True\<close>]; simp)
 
-lemma (in \<phi>min) op_get_var''_\<phi>app:
+lemma op_get_var''_\<phi>app:
    \<open>\<^bold>p\<^bold>r\<^bold>e\<^bold>m\<^bold>i\<^bold>s\<^bold>e v \<in> Well_Type TY
 \<Longrightarrow> \<^bold>p\<^bold>r\<^bold>o\<^bold>c op_get_var vname TY \<lbrace> v \<Ztypecolon> Var vname Identity \<longmapsto> v \<Ztypecolon> Var vname Identity \<heavy_comma> \<^bold>v\<^bold>a\<^bold>l v \<Ztypecolon> Identity \<rbrace>\<close>
   unfolding op_get_var_def Premise_def
   by (rule,assumption,rule,simp add: \<phi>expns)
 
-end
 
-
-lemma (in \<phi>min) op_set_var''_\<phi>app:
+lemma op_set_var''_\<phi>app:
    \<open>\<^bold>p\<^bold>r\<^bold>e\<^bold>m\<^bold>i\<^bold>s\<^bold>e v \<in> Well_Type TY
 \<Longrightarrow> \<^bold>p\<^bold>r\<^bold>e\<^bold>m\<^bold>i\<^bold>s\<^bold>e u \<in> Well_Type TY
 \<Longrightarrow> \<^bold>p\<^bold>r\<^bold>o\<^bold>c op_set_var vname TY rawv \<lbrace> v \<Ztypecolon> Var vname Identity\<heavy_comma> u \<Ztypecolon> Val rawv Identity \<longmapsto> u \<Ztypecolon> Var vname Identity \<rbrace>\<close>
   unfolding op_set_var_def Premise_def
   by (cases rawv; simp, rule, simp add: \<phi>expns, rule, assumption, simp add: \<phi>expns, rule)
 
-lemma (in \<phi>min) op_var_scope':
+lemma op_var_scope':
    \<open>\<^bold>p\<^bold>r\<^bold>e\<^bold>m\<^bold>i\<^bold>s\<^bold>e v \<in> Well_Type TY
 \<Longrightarrow> (\<And>vname. \<^bold>p\<^bold>r\<^bold>o\<^bold>c F vname \<lbrace> X\<heavy_comma> v \<Ztypecolon> Var vname Identity \<longmapsto> Y \<^bold>t\<^bold>h\<^bold>r\<^bold>o\<^bold>w\<^bold>s E \<rbrace> )
 \<Longrightarrow> \<^bold>p\<^bold>r\<^bold>o\<^bold>c op_var_scope' TY F rawv \<lbrace> X\<heavy_comma> v \<Ztypecolon> Val rawv Identity \<longmapsto> Y \<^bold>t\<^bold>h\<^bold>r\<^bold>o\<^bold>w\<^bold>s E \<rbrace>\<close>
@@ -689,7 +557,7 @@ lemma (in \<phi>min) op_var_scope':
   apply (cases rawv; simp, rule, simp add: \<phi>expns)
   apply (clarsimp simp add: \<phi>expns \<phi>Procedure_\<phi>Res_Spec simp del: set_mult_expn del: subsetI)
   subgoal for r res c
-  apply (rule R_var.\<phi>R_allocate_res_entry[where R="(\<I> F.INTERP (r * c))"])
+  apply (rule R_var.\<phi>R_allocate_res_entry[where R="(\<I> INTERP (r * c))"])
      apply (clarsimp) using finite_map_freshness infinite_varname apply blast
       apply (clarsimp)
 
@@ -697,13 +565,13 @@ lemma (in \<phi>min) op_var_scope':
   subgoal premises prems for k res'
     apply (rule prems(2)[THEN spec[where x=r], THEN spec[where x=res'],
                 simplified prems, simplified, THEN mp])
-    apply (rule exI[where x=\<open>c * F.FIC_var.mk (1(k \<mapsto> v))\<close>])
+    apply (rule exI[where x=\<open>c * FIC_var.mk (1(k \<mapsto> v))\<close>])
     apply (simp add: \<phi>expns prems)
-    by (smt (verit, ccfv_threshold) FIC_var.expand FIC_var.sep_disj_fiction Fic_Space_Un F.Fic_Space_m \<phi>Res_Spec_mult_homo prems(5) prems(6) prems(7) prems(8) prems(9) sep_disj_multD2 sep_disj_multI2 sep_mult_assoc')
+    by (smt (verit, ccfv_threshold) FIC_var.expand FIC_var.sep_disj_fiction Fic_Space_Un Fic_Space_m \<phi>Res_Spec_mult_homo prems(5) prems(6) prems(7) prems(8) prems(9) sep_disj_multD2 sep_disj_multI2 sep_mult_assoc')
   . .
 
 
-lemma (in \<phi>min) op_free_var:
+lemma op_free_var:
    \<open>\<^bold>p\<^bold>r\<^bold>o\<^bold>c op_free_var vname \<lbrace> v \<Ztypecolon> Var vname Identity \<longmapsto> 1 \<rbrace>\<close>
   unfolding op_free_var_def \<phi>Procedure_\<phi>Res_Spec
   by (clarsimp simp add: \<phi>expns FIC_var.expand  simp del: set_mult_expn del: subsetI;
@@ -712,43 +580,41 @@ lemma (in \<phi>min) op_free_var:
 
 subsection \<open>Branches & Loops\<close>
 
-context \<phi>min_sem begin
-
 paragraph \<open>Non-Branching Selection\<close>
 
-definition op_sel :: "'TY \<Rightarrow> ('VAL \<times> 'VAL \<times> 'VAL, 'VAL,'VAL,'RES_N,'RES) proc'"
+definition op_sel :: "TY \<Rightarrow> (VAL \<times> VAL \<times> VAL, VAL) proc'"
   where "op_sel TY =
     \<phi>M_caseV (\<lambda>vc. \<phi>M_caseV (\<lambda>va vb.
-    \<phi>M_getV (int 1) V.Int.dest vc (\<lambda>c.
+    \<phi>M_getV (int 1) V_int.dest vc (\<lambda>c.
     \<phi>M_getV TY id va (\<lambda>a.
     \<phi>M_getV TY id vb (\<lambda>b.
     Return (sem_value (if snd c = 1 then b else a)))))))"
 
 paragraph \<open>Branch\<close>
 
-definition op_if :: "('ret,'VAL,'RES_N,'RES) proc
-                  \<Rightarrow> ('ret,'VAL,'RES_N,'RES) proc
-                  \<Rightarrow> ('VAL,'ret,'VAL,'RES_N,'RES) proc'"
+definition op_if :: "'ret proc
+                  \<Rightarrow> 'ret proc
+                  \<Rightarrow> (VAL,'ret) proc'"
   where "op_if brT brF v =
-    \<phi>M_getV (int 1) V.Int.dest v (\<lambda>c. (if snd c = 1 then brT else brF))"
+    \<phi>M_getV (int 1) V_int.dest v (\<lambda>c. (if snd c = 1 then brT else brF))"
 
 paragraph \<open>While Loop\<close>
 
-inductive SemDoWhile :: "('VAL,'VAL,'RES_N,'RES) proc \<Rightarrow> ('RES_N \<Rightarrow> 'RES) \<Rightarrow> (unit,'VAL,'RES_N,'RES) state \<Rightarrow> bool" where
-  "Success (sem_value (V.Int.mk (1,0))) res \<in> f s \<Longrightarrow> SemDoWhile f s (Success (sem_value ()) res)"
-| "Success (sem_value (V.Int.mk (1,1))) res \<in> f s \<Longrightarrow> SemDoWhile f res s'' \<Longrightarrow> SemDoWhile f s s''"
+inductive SemDoWhile :: "VAL proc \<Rightarrow> resource \<Rightarrow> unit state \<Rightarrow> bool" where
+  "Success (sem_value (V_int.mk (1,0))) res \<in> f s \<Longrightarrow> SemDoWhile f s (Success (sem_value ()) res)"
+| "Success (sem_value (V_int.mk (1,1))) res \<in> f s \<Longrightarrow> SemDoWhile f res s'' \<Longrightarrow> SemDoWhile f s s''"
 | "Exception v e \<in> f s \<Longrightarrow> SemDoWhile f s (Exception v e)"
 | "PartialCorrect \<in> f s \<Longrightarrow> SemDoWhile f s PartialCorrect"
 | "Invalid \<in> f s \<Longrightarrow> SemDoWhile f s Invalid"
 
-lemma "\<nexists> y. SemDoWhile ((\<lambda>res. Return (sem_value (V.Int.mk (1,1))) res)::('VAL,'VAL,'RES_N,'RES) proc) res y"
+lemma "\<nexists> y. SemDoWhile ((\<lambda>res. Return (sem_value (V_int.mk (1,1))) res) :: VAL proc) res y"
   apply rule apply (elim exE) subgoal for y
-    apply (induct "((\<lambda>res. Return (sem_value (V.Int.mk (1,1))) (res::'RES_N \<Rightarrow> 'RES))::('VAL,'VAL,'RES_N,'RES) proc)" res y
+    apply (induct "((\<lambda>res. Return (sem_value (V_int.mk (1,1))) (res::resource)) :: VAL proc)" res y
            rule: SemDoWhile.induct)
        apply (simp_all add: Return_def det_lift_def) . .
 
-definition op_do_while :: "('VAL,'VAL,'RES_N,'RES) proc \<Rightarrow> (unit,'VAL,'RES_N,'RES) proc" where
-  "op_do_while f s = Collect (SemDoWhile f s)"
+definition op_do_while :: " VAL proc \<Rightarrow> unit proc"
+  where "op_do_while f s = Collect (SemDoWhile f s)"
 
 (* lemma SemDoWhile_deterministic:
   assumes "SemDoWhile c s s1"
@@ -769,19 +635,16 @@ lemma SemDoWhile_deterministic2:
 
 paragraph \<open>Recursion\<close>
 
-inductive SemRec :: "(('a,'a,'VAL,'RES_N,'RES) proc' \<Rightarrow> ('a,'a,'VAL,'RES_N,'RES) proc')
-            \<Rightarrow> 'a sem_value \<Rightarrow> ('RES_N \<Rightarrow> 'RES) \<Rightarrow> ('a,'VAL,'RES_N,'RES) state set \<Rightarrow> bool"
+inductive SemRec :: "(('a,'a) proc' \<Rightarrow> ('a,'a) proc')
+            \<Rightarrow> 'a sem_value \<Rightarrow> resource \<Rightarrow> 'a state set \<Rightarrow> bool"
 where
   SemRec_I0: "(\<And>g. F g x res = y) \<Longrightarrow> SemRec F x res y"
 | SemRec_IS: "SemRec (F o F) x res y \<Longrightarrow> SemRec F x res y"
 
-definition op_recursion :: "'TY list \<Rightarrow> 'TY list
-                         \<Rightarrow> (('a,'a,'VAL,'RES_N,'RES) proc' \<Rightarrow> ('a,'a,'VAL,'RES_N,'RES) proc')
-                         \<Rightarrow> ('a,'a,'VAL,'RES_N,'RES) proc'"
+definition op_recursion :: "TY list \<Rightarrow> TY list
+                         \<Rightarrow> (('a,'a) proc' \<Rightarrow> ('a,'a) proc')
+                         \<Rightarrow> ('a,'a) proc'"
   where "op_recursion _ _ F x s = (if (\<exists>t. SemRec F x s t) then The (SemRec F x s) else {})"
-
-
-end
 
 end
 
