Phi_System/Calculus_of_Programming.thy
@@ -38,12 +38,7 @@ give two modes \<open>programming_mode\<close> and \<open>view_shift_mode\<close
 consts programming_mode :: mode
        view_shift_mode  :: mode
 
-context \<phi>spec begin
-
-definition CurrentConstruction :: " mode
-                        \<Rightarrow> ('RES_N \<Rightarrow> 'RES)
-                        \<Rightarrow> ('FIC_N,'FIC) assn
-                        \<Rightarrow> ('FIC_N,'FIC) assn \<Rightarrow> bool "
+definition CurrentConstruction :: " mode \<Rightarrow> resource \<Rightarrow> assn \<Rightarrow> assn \<Rightarrow> bool "
   where "CurrentConstruction mode s R S \<longleftrightarrow> s \<in> (INTERP_SPEC (R * S))"
 
 abbreviation Programming_CurrentConstruction ("\<^bold>c\<^bold>u\<^bold>r\<^bold>r\<^bold>e\<^bold>n\<^bold>t _ [_]/ \<^bold>r\<^bold>e\<^bold>s\<^bold>u\<^bold>l\<^bold>t\<^bold>s \<^bold>i\<^bold>n _" [1000,1000,11] 10)
@@ -52,12 +47,12 @@ abbreviation Programming_CurrentConstruction ("\<^bold>c\<^bold>u\<^bold>r\<^bol
 abbreviation View_Shift_CurrentConstruction ("\<^bold>v\<^bold>i\<^bold>e\<^bold>w _ [_]/ \<^bold>i\<^bold>s _" [1000,1000,11] 10)
   where \<open>View_Shift_CurrentConstruction \<equiv> CurrentConstruction view_shift_mode\<close>
 
-definition PendingConstruction :: " ('ret,'ex,'RES_N,'RES) proc
-                        \<Rightarrow> ('RES_N \<Rightarrow> 'RES)
-                        \<Rightarrow> ('FIC_N,'FIC) assn
-                        \<Rightarrow> ('ret sem_value \<Rightarrow> ('FIC_N,'FIC) assn)
-                        \<Rightarrow> ('ex sem_value \<Rightarrow> ('FIC_N,'FIC) assn)
-                        \<Rightarrow> bool "
+definition PendingConstruction :: " 'ret proc
+                                  \<Rightarrow> resource
+                                  \<Rightarrow> assn
+                                  \<Rightarrow> ('ret sem_value \<Rightarrow> assn)
+                                  \<Rightarrow> (VAL sem_value \<Rightarrow> assn)
+                                  \<Rightarrow> bool "
     ("\<^bold>p\<^bold>e\<^bold>n\<^bold>d\<^bold>i\<^bold>n\<^bold>g _ \<^bold>o\<^bold>n _ [_]/ \<^bold>r\<^bold>e\<^bold>s\<^bold>u\<^bold>l\<^bold>t\<^bold>s \<^bold>i\<^bold>n _/ \<^bold>t\<^bold>h\<^bold>r\<^bold>o\<^bold>w\<^bold>s _" [1000,1000,1000,11,11] 10)
     where "PendingConstruction f s R S E \<longleftrightarrow> f s \<subseteq> \<S> (\<lambda>ret. INTERP_SPEC (R * S ret)) (\<lambda>ex. INTERP_SPEC (R * E ex))"
 
@@ -65,8 +60,6 @@ definition \<open>CodeBlock s s' f ret \<longleftrightarrow> Success ret s' \<in
 
 lemma CurrentConstruction_D: "CurrentConstruction mode s H T \<Longrightarrow> Inhabited T"
   unfolding CurrentConstruction_def Inhabited_def by (clarsimp simp add: \<phi>expns; blast)
-
-end
 
 
 subsection \<open>Forward Declaration of Reasoner\<close>
@@ -106,15 +99,12 @@ unchanged.
   \<^term>\<open>X\<^sub>j\<close> that unifies \<^term>\<open>Y\<^sub>i\<close>.
 \<close>
 
-lemma (in \<phi>spec)
-  [\<phi>reason 3000 for \<open>\<^bold>v\<^bold>i\<^bold>e\<^bold>w ?X \<longmapsto> ?X' \<^bold>w\<^bold>i\<^bold>t\<^bold>h ?P \<^bold><\<^bold>a\<^bold>c\<^bold>t\<^bold>i\<^bold>o\<^bold>n\<^bold>> ToSA' ?mode\<close>]:
+lemma [\<phi>reason 3000 for \<open>\<^bold>v\<^bold>i\<^bold>e\<^bold>w ?X \<longmapsto> ?X' \<^bold>w\<^bold>i\<^bold>t\<^bold>h ?P \<^bold><\<^bold>a\<^bold>c\<^bold>t\<^bold>i\<^bold>o\<^bold>n\<^bold>> ToSA' ?mode\<close>]:
   \<open>\<^bold>v\<^bold>i\<^bold>e\<^bold>w X \<longmapsto> X \<^bold><\<^bold>a\<^bold>c\<^bold>t\<^bold>i\<^bold>o\<^bold>n\<^bold>> ToSA' mode\<close>
   unfolding Action_Tag_def using \<phi>view_refl .
 
 
 subsection \<open>Rules for Constructing Programs\<close>
-
-context \<phi>spec begin
 
 subsubsection \<open>Construct Procedure\<close>
 
@@ -137,11 +127,11 @@ lemma
 \<^bold>p\<^bold>e\<^bold>n\<^bold>d\<^bold>i\<^bold>n\<^bold>g f \<^bold>o\<^bold>n s [R] \<^bold>r\<^bold>e\<^bold>s\<^bold>u\<^bold>l\<^bold>t\<^bold>s \<^bold>i\<^bold>n U \<^bold>t\<^bold>h\<^bold>r\<^bold>o\<^bold>w\<^bold>s E1 \<longrightarrow> 
   Invalid \<notin> f s \<and> (\<forall>v s'. Exception v s' \<in> f s \<longrightarrow> s' \<in> INTERP_SPEC (R \<heavy_comma> E v))*)
 
-lemma (in \<phi>empty) \<phi>assemble_proc:
+lemma \<phi>assemble_proc:
   \<open> \<^bold>p\<^bold>e\<^bold>n\<^bold>d\<^bold>i\<^bold>n\<^bold>g f \<^bold>o\<^bold>n s [R] \<^bold>r\<^bold>e\<^bold>s\<^bold>u\<^bold>l\<^bold>t\<^bold>s \<^bold>i\<^bold>n T \<^bold>t\<^bold>h\<^bold>r\<^bold>o\<^bold>w\<^bold>s E1
 \<Longrightarrow> (\<And>s' ret. CodeBlock s s' f ret \<Longrightarrow> \<^bold>p\<^bold>e\<^bold>n\<^bold>d\<^bold>i\<^bold>n\<^bold>g (g ret) \<^bold>o\<^bold>n s' [R] \<^bold>r\<^bold>e\<^bold>s\<^bold>u\<^bold>l\<^bold>t\<^bold>s \<^bold>i\<^bold>n U \<^bold>t\<^bold>h\<^bold>r\<^bold>o\<^bold>w\<^bold>s E2)
 \<Longrightarrow> \<^bold>p\<^bold>e\<^bold>n\<^bold>d\<^bold>i\<^bold>n\<^bold>g (f \<bind> g) \<^bold>o\<^bold>n s [R] \<^bold>r\<^bold>e\<^bold>s\<^bold>u\<^bold>l\<^bold>t\<^bold>s \<^bold>i\<^bold>n U \<^bold>t\<^bold>h\<^bold>r\<^bold>o\<^bold>w\<^bold>s E1 + E2\<close>
-  for E1 :: \<open>'VAL sem_value \<Rightarrow> ('FIC_N \<Rightarrow> 'FIC) set\<close>
+  for E1 :: \<open>VAL sem_value \<Rightarrow> assn\<close>
   unfolding CurrentConstruction_def PendingConstruction_def bind_def subset_iff CodeBlock_def
   apply clarsimp subgoal for s s'
   by (cases s; simp; cases s'; simp add: split_state_All ring_distribs plus_fun) .
@@ -163,7 +153,7 @@ lemma \<phi>accept_proc:
 lemma \<phi>return_when_unreachable:
   \<open> \<^bold>p\<^bold>e\<^bold>n\<^bold>d\<^bold>i\<^bold>n\<^bold>g f \<^bold>o\<^bold>n s [R] \<^bold>r\<^bold>e\<^bold>s\<^bold>u\<^bold>l\<^bold>t\<^bold>s \<^bold>i\<^bold>n (\<lambda>_. T) \<^bold>t\<^bold>h\<^bold>r\<^bold>o\<^bold>w\<^bold>s E
 \<Longrightarrow> \<^bold>p\<^bold>e\<^bold>n\<^bold>d\<^bold>i\<^bold>n\<^bold>g (f \<ggreater> Return (sem_value undefined)) \<^bold>o\<^bold>n s [R] \<^bold>r\<^bold>e\<^bold>s\<^bold>u\<^bold>l\<^bold>t\<^bold>s \<^bold>i\<^bold>n (\<lambda>_. T) \<^bold>t\<^bold>h\<^bold>r\<^bold>o\<^bold>w\<^bold>s E\<close>
-  for f :: \<open>(unreachable, 'ex, 'RES_N, 'RES) proc\<close>
+  for f :: \<open>unreachable proc\<close>
   unfolding CurrentConstruction_def PendingConstruction_def bind_def Return_def det_lift_def subset_iff
   apply clarsimp subgoal for s' s'' by (cases s'; simp; cases s''; simp add: ring_distribs; blast) .
 
@@ -284,7 +274,7 @@ lemma "_\<phi>cast_exception_rule_":
   using "_\<phi>cast_exception_" .
 
 
-lemma (in -) "_\<phi>cast_implication_":
+lemma "_\<phi>cast_implication_":
   \<open> x \<in> S
 \<Longrightarrow> S \<^bold>i\<^bold>m\<^bold>p\<^bold>l\<^bold>i\<^bold>e\<^bold>s T \<^bold>a\<^bold>n\<^bold>d Any \<^bold><\<^bold>a\<^bold>c\<^bold>t\<^bold>i\<^bold>o\<^bold>n\<^bold>> ToSA
 \<Longrightarrow> \<r>Success
@@ -296,7 +286,7 @@ subsubsection \<open>Misc\<close>
 
 paragraph \<open>Inhabitance\<close>
 
-lemma (in -) Implication_Inhabited_rule:
+lemma Implication_Inhabited_rule:
   \<open>x \<in> S \<Longrightarrow> (Inhabited S \<Longrightarrow> C) \<Longrightarrow> C\<close>
   unfolding Inhabited_def by blast
 
@@ -322,9 +312,9 @@ lemma [simp]:
   "(CurrentConstruction mode s H T \<and> B) \<and> C \<longleftrightarrow> (CurrentConstruction mode s H T) \<and> (B \<and> C)"
   by simp
 
-declare (in -) Subjection_expn[\<phi>programming_simps]
+declare Subjection_expn[\<phi>programming_simps]
 
-lemma (in -) [\<phi>programming_simps]:
+lemma [\<phi>programming_simps]:
   \<open>((s \<in> T) \<and> B) \<and> C \<longleftrightarrow> (s \<in> T) \<and> (B \<and> C)\<close>
   by simp
 
@@ -360,7 +350,6 @@ lemma Subjection_simp_proc_arg:
 
 lemmas Subjection_simp_proc_arg_metaeq[unfolded atomize_eq[symmetric]] = Subjection_simp_proc_arg
 
-end
 
 subsection \<open>Primitive \<phi>-Types\<close>
 
@@ -385,20 +374,11 @@ consts anonymous :: 'a
 
 syntax val_syntax :: "logic \<Rightarrow> logic" ("\<^bold>v\<^bold>a\<^bold>l _" [18] 17)
 
-setup \<open>(Sign.add_trrules (let open Ast 
-    in [
-      Syntax.Parse_Rule (
-        Appl [Constant \<^syntax_const>\<open>val_syntax\<close>,
-                Appl [Constant \<^const_syntax>\<open>\<phi>Type\<close>, Variable "x", Variable "T"]],
-        Appl [Constant \<^const_syntax>\<open>\<phi>Type\<close>, Variable "x",
-                Appl [Constant \<^const_syntax>\<open>Val\<close>, Constant \<^const_name>\<open>anonymous\<close>, Variable "T"]])
-  ] end))\<close>
+translations "\<^bold>v\<^bold>a\<^bold>l (x \<Ztypecolon> T)" => "x \<Ztypecolon> CONST Val (CONST anonymous) T"
 
-term \<open>\<^bold>v\<^bold>a\<^bold>l x \<Ztypecolon> T\<close>
-term \<open>x \<Ztypecolon> \<^bold>v\<^bold>a\<^bold>l[AA] Y\<close>
+declare [ [ML_debugger]]
 
 ML_file \<open>library/procedure_syntax.ML\<close>
-
 
 
 end
